devel/Iron/SystemF2Effect/Base.v
@@ -4,7 +4,7 @@ Require Export Iron.Data.List.
 Require Export Iron.Data.Nat.
 Require Export Iron.Norm.List.
 Require Export Iron.Norm.
-Require Export Iron.Tactics.Rip2.
+Require Export Iron.Tactics.Rip3.
 Require Export Iron.Tactics.Rewrite2.
 Require Export Iron.Tactics.Case.
 Require Export Iron.Tactics.Nope.
@@ -16,6 +16,14 @@ Require Export Iron.Tactics.LibTactics.
 Require Export Coq.Arith.Arith.
 Require Export Coq.Arith.Compare_dec.
 Require Export Coq.Logic.FunctionalExtensionality.
+
+
+(* Comparisons on nats are common when using deBruijn indices.
+   Automatically try the omega tactic when we see one. *)
+Hint Extern 4 (_ >  _) => omega.
+Hint Extern 4 (_ <  _) => omega.
+Hint Extern 4 (_ >= _) => omega.
+Hint Extern 4 (_ <= _) => omega.
 
 
 (* The norm_beq_nat tactic normalises this,
@@ -56,11 +64,13 @@ Tactic Notation "burn0" "using" tactic(T)
 
 Tactic Notation "burn"
  := try (solve [ burn0
-               | red; burn0 ]).
+               | red; burn0
+               | repeat f_equal; burn0 ]).
 
 Tactic Notation "burn" "using" tactic(T) 
  := try (solve [ burn0 using T
-               | red; burn0 using T]).
+               | red; burn0 using T
+               | repeat f_equal; burn0 using T ]).
 
 
 Ltac have_auto ::= burn.
